compiler/conLangScript.sml
@@ -18,13 +18,12 @@ val _ = new_theory "conLang"
  * name environment.
  *
  * The semantics of IL2 differ in that there is no constructor name
- * environment, and pattern matches that fall off the end give a type error.
+ * environment.
  *
  * The translator to IL2 keeps a mapping of constructors to their tags. The
  * tuple constructor is always 0. Div, Bind, and Eq are always 1, 2, and 3.
  * Cond and nil are always 4 and 5. It also keeps a reverse mapping for use by
- * the REPL printer. It also adds an extra case to non-exhaustive pattern
- * matches. At the moment, it just adds the default case to all matches.
+ * the REPL printer. 
  *
  * The expressions include the unary operation for initialising the global
  * store, even though it can't be used until IL3. However, including it here
@@ -71,6 +70,8 @@ val _ = Define `
  (nil_tag =( 5))`;
 
 
+val _ = type_abbrev( "exh_ctors_env" , ``: (( typeN id), ( num list)) fmap``);
+
 val _ = Hol_datatype `
  uop_i2 = 
     Opderef_i2
@@ -82,7 +83,7 @@ val _ = Hol_datatype `
  pat_i2 =
     Pvar_i2 of varN
   | Plit_i2 of lit
-  | Pcon_i2 of num => pat_i2 list
+  | Pcon_i2 of (num #  tid_or_exn option) => pat_i2 list
   | Pref_i2 of pat_i2`;
 
 
@@ -91,7 +92,7 @@ val _ = Hol_datatype `
     Raise_i2 of exp_i2
   | Handle_i2 of exp_i2 => (pat_i2 # exp_i2) list
   | Lit_i2 of lit
-  | Con_i2 of num => exp_i2 list
+  | Con_i2 of (num #  tid_or_exn option) => exp_i2 list
   | Var_local_i2 of varN
   | Var_global_i2 of num
   | Fun_i2 of varN => exp_i2
@@ -118,7 +119,7 @@ val _ = Hol_datatype `
 val _ = Hol_datatype `
  v_i2 =
     Litv_i2 of lit
-  | Conv_i2 of num => v_i2 list 
+  | Conv_i2 of (num #  tid_or_exn option) => v_i2 list 
   | Closure_i2 of (varN, v_i2) env => varN => exp_i2
   | Recclosure_i2 of (varN, v_i2) env => (varN # varN # exp_i2) list => varN
   | Loc_i2 of num`;
@@ -149,27 +150,27 @@ val _ = Lib.with_flag (computeLib.auto_import_definitions, false) Defn.save_defn
 
 (* Maps a constructor name to its tag and to all of the constructor names of
  * its type, for use in exhaustiveness checking *)
-val _ = type_abbrev( "flat_tag_env" , ``: (conN, (num #  ( conN list)option)) fmap``);
+val _ = type_abbrev( "flat_tag_env" , ``: (conN, (num #  tid_or_exn option)) fmap``);
 val _ = type_abbrev( "tag_env" , ``: (modN, flat_tag_env) fmap # flat_tag_env``);
 
-(*val lookup_tag_flat : conN -> flat_tag_env -> (nat * maybe (list conN))*)
+(*val lookup_tag_flat : conN -> flat_tag_env -> (nat * maybe tid_or_exn)*)
 val _ = Define `
  (lookup_tag_flat cn ftagenv =  
 ((case FLOOKUP ftagenv cn of
-      NONE => (tuple_tag, SOME [])
+      NONE => (tuple_tag, NONE)
     | SOME (n,ctors) => (n,ctors)
   )))`;
 
 
-(*val lookup_tag_env : maybe (id conN) -> tag_env -> (nat * maybe (list conN))*)
+(*val lookup_tag_env : maybe (id conN) -> tag_env -> (nat * maybe tid_or_exn)*)
 val _ = Define `
  (lookup_tag_env id (mtagenv,tagenv) =  
 ((case id of
-      NONE => (tuple_tag, SOME [])
+      NONE => (tuple_tag,NONE) 
     | SOME (Short x) => lookup_tag_flat x tagenv
     | SOME (Long x y) =>
         (case FLOOKUP mtagenv x of
-            NONE => (tuple_tag, SOME [])
+            NONE => (tuple_tag,NONE) 
           | SOME tagenv => lookup_tag_flat y tagenv
         )
   )))`;
@@ -183,7 +184,7 @@ val _ = Define `
 (pat_to_i2 tagenv (Plit l) = (Plit_i2 l))
 /\ 
 (pat_to_i2 tagenv (Pcon con_id ps) =  
- (Pcon_i2 (FST (lookup_tag_env con_id tagenv)) (MAP (pat_to_i2 tagenv) ps)))
+ (Pcon_i2 (lookup_tag_env con_id tagenv) (MAP (pat_to_i2 tagenv) ps)))
 /\ 
 (pat_to_i2 tagenv (Pref p) = (Pref_i2 (pat_to_i2 tagenv p)))`;
 
@@ -198,61 +199,6 @@ val _ = Define `
   )))`;
 
 
-(*val is_pvar : pat -> bool*)
-val _ = Define `
- (is_pvar p =  
-((case p of
-      Pvar _ => T
-    | _ => F
-  )))`;
-
-
-(*
-val get_pcons : list pat -> maybe (list conN)
-let rec get_pcons [] = Just []
-and get_pcons (p::ps) =
-  match p with
-    | Pcon c ps' ->
-        if List.all is_pvar ps' then
-          match get_pcons ps with
-            | Nothing -> Nothing
-            | Just cons -> Just (id_to_n c::cons)
-          end
-        else
-          Nothing
-    | _ -> Nothing
-  end
-
-val exhaustive_match : tag_env -> list pat -> bool
-let exhaustive_match tagenv ps =
-  match ps with
-    | [Pvar _] -> true
-    | (Pcon c ps'::ps) ->
-      match get_pcons tagenv (Pcon c ps'::ps) with
-          Nothing -> false
-        | Just [] -> false
-        | Just tags -> 
-            Set.fromList (snd (lookup_tag_env c tagenv)) = Set.fromList tags
-      end
-  end
-*)
-
-(*val exhaustive_match : tag_env -> list pat -> bool*)
-val _ = Define `
- (exhaustive_match tagenv ps =
-  F)`;
-
-
-(*val add_default_case : bool -> bool -> list (pat_i2 * exp_i2) -> list (pat_i2 * exp_i2)*)
-val _ = Define `
- (add_default_case is_handle is_exhaustive pes =  
-(if is_exhaustive then
-    pes
-  else
-    let exp = (if is_handle then Var_local_i2 "x" else Con_i2 bind_tag []) in
-    pes ++ [(Pvar_i2 "x", Raise_i2 exp)]))`;
-
-
 (*val exp_to_i2 : tag_env -> exp_i1 -> exp_i2*)
 (*val exps_to_i2 : tag_env -> list exp_i1 -> list exp_i2*)
 (*val pat_exp_to_i2 : tag_env -> list (pat * exp_i1) -> list (pat_i2 * exp_i2)*)
@@ -263,13 +209,13 @@ val _ = Define `
  (Raise_i2 (exp_to_i2 tagenv e)))
 /\
 (exp_to_i2 tagenv (Handle_i1 e pes) =  
- (Handle_i2 (exp_to_i2 tagenv e) (add_default_case T (exhaustive_match tagenv (MAP FST pes)) (pat_exp_to_i2 tagenv pes))))
+ (Handle_i2 (exp_to_i2 tagenv e) (pat_exp_to_i2 tagenv pes)))
 /\
 (exp_to_i2 tagenv (Lit_i1 l) =  
  (Lit_i2 l)) 
 /\
 (exp_to_i2 tagenv (Con_i1 cn es) =  
- (Con_i2 (FST (lookup_tag_env cn tagenv)) (exps_to_i2 tagenv es)))
+ (Con_i2 (lookup_tag_env cn tagenv) (exps_to_i2 tagenv es)))
 /\
 (exp_to_i2 tagenv (Var_local_i1 x) = (Var_local_i2 x))
 /\
@@ -288,7 +234,7 @@ val _ = Define `
 (If_i2 (exp_to_i2 tagenv e1) (exp_to_i2 tagenv e2) (exp_to_i2 tagenv e3)))
 /\
 (exp_to_i2 tagenv (Mat_i1 e pes) =  
-(Mat_i2 (exp_to_i2 tagenv e) (add_default_case F (exhaustive_match tagenv (MAP FST pes)) (pat_exp_to_i2 tagenv pes))))
+(Mat_i2 (exp_to_i2 tagenv e) (pat_exp_to_i2 tagenv pes)))
 /\
 (exp_to_i2 tagenv (Let_i1 x e1 e2) =  
 (Let_i2 x (exp_to_i2 tagenv e1) (exp_to_i2 tagenv e2)))
@@ -316,22 +262,22 @@ val _ = Lib.with_flag (computeLib.auto_import_definitions, false) Defn.save_defn
 
 (* The constructor names that are in scope, the global mapping of constructor
  * names (with types so that they are unique), and its inverse. *)
-val _ = type_abbrev( "tagenv_state" , ``: num # tag_env # (num, (conN # tid_or_exn)) fmap # (conN # (num #  ( conN list)option)) list``);
+val _ = type_abbrev( "tagenv_state" , ``: num # tag_env # (num, (conN # tid_or_exn)) fmap # (conN # (num #  tid_or_exn option)) list``);
 
 val _ = Define `
  (get_tagenv (next,tagenv,inv0,acc) = tagenv)`;
 
 
-(*val insert_tag_env : conN -> (nat * maybe (list conN)) -> tag_env  -> tag_env*)
+(*val insert_tag_env : conN -> (nat * maybe tid_or_exn) -> tag_env  -> tag_env*)
 val _ = Define `
  (insert_tag_env cn tag (mtagenv,ftagenv) =
   (mtagenv,ftagenv |+ (cn, tag)))`;
 
 
-(*val alloc_tag : maybe (list conN) -> tid_or_exn -> conN -> tagenv_state -> tagenv_state*)
+(*val alloc_tag : tid_or_exn -> conN -> tagenv_state -> tagenv_state*)
 val _ = Define `
- (alloc_tag all_ctors tn cn (next,tagenv,inv0,acc) =
-  ((next+ 1),insert_tag_env cn (next,all_ctors) tagenv,inv0 |+ (next, (cn,tn)), ((cn,(next,all_ctors))::acc)))`;
+ (alloc_tag tn cn (next,tagenv,inv0,acc) =
+  ((next+ 1),insert_tag_env cn (next,SOME tn) tagenv,inv0 |+ (next, (cn,tn)), ((cn,(next,SOME tn))::acc)))`;
 
 
 (*val alloc_tags : maybe modN -> tagenv_state -> type_def -> tagenv_state*)
@@ -340,9 +286,8 @@ val _ = Define `
 (alloc_tags mn st [] = st)
 /\
 (alloc_tags mn st ((tvs,tn,constrs)::types) =  
- (let all_constrs = (SOME (MAP (\ (cn,ts) .  cn) constrs)) in
-  let st' =    
-(FOLDL (\ st' (cn,ts) .  alloc_tag all_constrs (TypeId (mk_id mn tn)) cn st') st constrs)
+ (let st' =    
+(FOLDL (\ st' (cn,ts) .  alloc_tag (TypeId (mk_id mn tn)) cn st') st constrs)
   in
     alloc_tags mn st' types))`;
 
@@ -363,11 +308,11 @@ val _ = Define `
     | Dtype_i1 mn type_def =>
         decs_to_i2 (alloc_tags mn st type_def) ds
     | Dexn_i1 mn cn ts =>
-        decs_to_i2 (alloc_tag NONE (TypeExn (mk_id mn cn)) cn st) ds
+        decs_to_i2 (alloc_tag (TypeExn (mk_id mn cn)) cn st) ds
   )))`;
 
 
-(*val mod_tagenv : maybe modN -> list (conN * (nat * maybe (list conN))) -> tag_env -> tag_env*)
+(*val mod_tagenv : maybe modN -> list (conN * (nat * maybe tid_or_exn)) -> tag_env -> tag_env*)
 val _ = Define `
  (mod_tagenv mn l (mtagenv,tagenv) =  
 ((case mn of
@@ -467,13 +412,13 @@ val _ = Define `
 
 val _ = Lib.with_flag (computeLib.auto_import_definitions, false) Defn.save_defn do_eq_i2_defn;
 
-val _ = type_abbrev( "all_env_i2" , ``: ( ( v_i2 option)list # (varN, v_i2) env)``);
+val _ = type_abbrev( "all_env_i2" , ``: (exh_ctors_env # ( v_i2 option) list # (varN, v_i2) env)``);
 
 val _ = Define `
- (all_env_i2_to_genv (genv,env) = genv)`;
+ (all_env_i2_to_genv (exh,genv,env) = genv)`;
 
 val _ = Define `
- (all_env_i2_to_env (genv,env) = env)`;
+ (all_env_i2_to_env (exh,genv,env) = env)`;
 
 
 (*val exn_env_i2 : env varN v_i2*)
@@ -494,7 +439,7 @@ val _ = Define `
         )
     | (Opn op, Litv_i2 (IntLit n1), Litv_i2 (IntLit n2)) =>
         if ((op = Divide) \/ (op = Modulo)) /\ (n2 =( 0 : int)) then
-          SOME (exn_env_i2, s, Raise_i2 (Con_i2 div_tag []))
+          SOME (exn_env_i2, s, Raise_i2 (Con_i2 (div_tag,SOME (TypeExn (Short "Div"))) []))
         else
           SOME (env', s, Lit_i2 (IntLit (opn_lookup op n1 n2)))
     | (Opb op, Litv_i2 (IntLit n1), Litv_i2 (IntLit n2)) =>
@@ -502,7 +447,7 @@ val _ = Define `
     | (Equality, v1, v2) =>
         (case do_eq_i2 v1 v2 of
             Eq_type_error => NONE
-          | Eq_closure => SOME (exn_env_i2, s, Raise_i2 (Con_i2 eq_tag []))
+          | Eq_closure => SOME (exn_env_i2, s, Raise_i2 (Con_i2 (eq_tag,SOME (TypeExn (Short "Exn"))) []))
           | Eq_val b => SOME (env', s, Lit_i2 (Bool b))
         )
     | (Opassign, (Loc_i2 lnum), v) =>
@@ -525,12 +470,12 @@ val _ = Define `
     NONE))`;
 
 
-(*val pmatch_i2 : store v_i2 -> pat_i2 -> v_i2 -> env varN v_i2 -> match_result (env varN v_i2)*)
+(*val pmatch_i2 : exh_ctors_env -> store v_i2 -> pat_i2 -> v_i2 -> env varN v_i2 -> match_result (env varN v_i2)*)
  val pmatch_i2_defn = Hol_defn "pmatch_i2" `
 
-(pmatch_i2 s (Pvar_i2 x) v' env = (Match (bind x v' env)))
+(pmatch_i2 exh s (Pvar_i2 x) v' env = (Match (bind x v' env)))
 /\
-(pmatch_i2 s (Plit_i2 l) (Litv_i2 l') env =  
+(pmatch_i2 exh s (Plit_i2 l) (Litv_i2 l') env =  
 (if l = l' then
     Match env
   else if lit_same_type l l' then
@@ -538,35 +483,58 @@ val _ = Define `
   else
     Match_type_error))
 /\
-(pmatch_i2 s (Pcon_i2 tag1 ps) (Conv_i2 tag2 vs) env =  
-(if tag1 = tag2 then
-    if LENGTH ps = LENGTH vs then
-      pmatch_list_i2 s ps vs env
-    else 
-      Match_type_error
+(pmatch_i2 exh s (Pcon_i2 (n, SOME (TypeExn _)) ps) (Conv_i2 (n', SOME (TypeExn _)) vs) env =  
+(if LENGTH ps = LENGTH vs then
+    if n = n' then
+      pmatch_list_i2 exh s ps vs env
+    else
+      No_match
   else
-    No_match))
+    Match_type_error))
 /\
-(pmatch_i2 s (Pref_i2 p) (Loc_i2 lnum) env =  
+(pmatch_i2 exh s (Pcon_i2 (n, SOME (TypeId t)) ps) (Conv_i2 (n', SOME (TypeId t')) vs) env =  
+(if (t = t') /\ (LENGTH ps = LENGTH vs) then
+    (case FLOOKUP exh t of
+        NONE => Match_type_error
+      | SOME tags =>
+          if MEM n tags /\ MEM n' tags then
+            if n = n' then
+              pmatch_list_i2 exh s ps vs env
+            else
+	      No_match
+          else
+            Match_type_error
+    )
+  else
+    Match_type_error))
+/\
+(pmatch_i2 exh s (Pcon_i2 (n,NONE) ps) (Conv_i2 (n',NONE) vs) env =  
+(if (LENGTH ps = LENGTH vs) /\ ((n = tuple_tag) /\ (n' = tuple_tag)) then
+    pmatch_list_i2 exh s ps vs env
+  else
+    Match_type_error))
+/\
+(pmatch_i2 exh s (Pref_i2 p) (Loc_i2 lnum) env =  
 ((case store_lookup lnum s of
-      SOME v => pmatch_i2 s p v env
+      SOME v => pmatch_i2 exh s p v env
     | NONE => Match_type_error
   )))
 /\
-(pmatch_i2 _ _ _ env = Match_type_error)
+(pmatch_i2 exh _ _ _ env = Match_type_error)
 /\
-(pmatch_list_i2 s [] [] env = (Match env))
+(pmatch_list_i2 exh s [] [] env = (Match env))
 /\
-(pmatch_list_i2 s (p::ps) (v::vs) env =  
-((case pmatch_i2 s p v env of
+(pmatch_list_i2 exh s (p::ps) (v::vs) env =  
+((case pmatch_i2 exh s p v env of
       No_match => No_match
     | Match_type_error => Match_type_error
-    | Match env' => pmatch_list_i2 s ps vs env'
+    | Match env' => pmatch_list_i2 exh s ps vs env'
   )))
 /\
-(pmatch_list_i2 s _ _ env = Match_type_error)`;
+(pmatch_list_i2 exh s _ _ env = Match_type_error)`;
 
 val _ = Lib.with_flag (computeLib.auto_import_definitions, false) Defn.save_defn pmatch_i2_defn;
+
 
 val _ = Hol_reln ` (! ck env l s.
 T
@@ -590,7 +558,7 @@ evaluate_i2 ck s1 env (Handle_i2 e pes) (s2, Rval v))
 
 /\ (! ck s1 s2 env e pes v bv.
 (evaluate_i2 ck env s1 e (s2, Rerr (Rraise v)) /\
-evaluate_match_i2 ck env s2 v pes bv)
+evaluate_match_i2 ck env s2 v pes v bv)
 ==>
 evaluate_i2 ck env s1 (Handle_i2 e pes) bv)
 
@@ -659,31 +627,31 @@ evaluate_i2 ck env s1 (Uapp_i2 uop e) ((count,s2), Rerr Rtype_error))
 ==>
 evaluate_i2 ck env s (Uapp_i2 uop e) (s', Rerr err))
 
-/\ (! ck genv env op e1 e2 v1 v2 env' e3 bv s1 s2 s3 count s4.
-(evaluate_i2 ck (genv,env) s1 e1 (s2, Rval v1) /\
-(evaluate_i2 ck (genv,env) s2 e2 ((count,s3), Rval v2) /\
+/\ (! ck exh genv env op e1 e2 v1 v2 env' e3 bv s1 s2 s3 count s4.
+(evaluate_i2 ck (exh,genv,env) s1 e1 (s2, Rval v1) /\
+(evaluate_i2 ck (exh,genv,env) s2 e2 ((count,s3), Rval v2) /\
 ((do_app_i2 env s3 op v1 v2 = SOME (env', s4, e3)) /\
 (((ck /\ (op = Opapp)) ==> ~ (count =( 0))) /\
-evaluate_i2 ck (genv,env') ((if ck then dec_count op count else count),s4) e3 bv))))
+evaluate_i2 ck (exh,genv,env') ((if ck then dec_count op count else count),s4) e3 bv))))
 ==>
-evaluate_i2 ck (genv,env) s1 (App_i2 op e1 e2) bv)
+evaluate_i2 ck (exh,genv,env) s1 (App_i2 op e1 e2) bv)
 
-/\ (! ck genv env op e1 e2 v1 v2 env' e3 s1 s2 s3 count s4.
-(evaluate_i2 ck (genv,env) s1 e1 (s2, Rval v1) /\
-(evaluate_i2 ck (genv,env) s2 e2 ((count,s3), Rval v2) /\
+/\ (! ck exh genv env op e1 e2 v1 v2 env' e3 s1 s2 s3 count s4.
+(evaluate_i2 ck (exh,genv,env) s1 e1 (s2, Rval v1) /\
+(evaluate_i2 ck (exh,genv,env) s2 e2 ((count,s3), Rval v2) /\
 ((do_app_i2 env s3 op v1 v2 = SOME (env', s4, e3)) /\
 ((count = 0) /\
 ((op = Opapp) /\
 ck)))))
 ==>
-evaluate_i2 ck (genv,env) s1 (App_i2 op e1 e2) (( 0,s4), Rerr Rtimeout_error))
+evaluate_i2 ck (exh,genv,env) s1 (App_i2 op e1 e2) (( 0,s4), Rerr Rtimeout_error))
 
-/\ (! ck genv env op e1 e2 v1 v2 s1 s2 s3 count.
-(evaluate_i2 ck (genv,env) s1 e1 (s2, Rval v1) /\
-(evaluate_i2 ck (genv,env) s2 e2 ((count,s3), Rval v2) /\
+/\ (! ck exh genv env op e1 e2 v1 v2 s1 s2 s3 count.
+(evaluate_i2 ck (exh,genv,env) s1 e1 (s2, Rval v1) /\
+(evaluate_i2 ck (exh,genv,env) s2 e2 ((count,s3), Rval v2) /\
 (do_app_i2 env s3 op v1 v2 = NONE)))
 ==>
-evaluate_i2 ck (genv,env) s1 (App_i2 op e1 e2) ((count,s3), Rerr Rtype_error))
+evaluate_i2 ck (exh,genv,env) s1 (App_i2 op e1 e2) ((count,s3), Rerr Rtype_error))
 
 /\ (! ck env op e1 e2 v1 err s1 s2 s3.
 (evaluate_i2 ck env s1 e1 (s2, Rval v1) /\
@@ -716,7 +684,7 @@ evaluate_i2 ck env s (If_i2 e1 e2 e3) (s', Rerr err))
 
 /\ (! ck env e pes v bv s1 s2.
 (evaluate_i2 ck env s1 e (s2, Rval v) /\
-evaluate_match_i2 ck env s2 v pes bv)
+evaluate_match_i2 ck env s2 v pes (Conv_i2 (bind_tag,SOME (TypeExn (Short "Bind"))) []) bv)
 ==>
 evaluate_i2 ck env s1 (Mat_i2 e pes) bv)
 
@@ -725,22 +693,22 @@ evaluate_i2 ck env s1 (Mat_i2 e pes) bv)
 ==>
 evaluate_i2 ck env s (Mat_i2 e pes) (s', Rerr err))
 
-/\ (! ck genv env n e1 e2 v bv s1 s2.
-(evaluate_i2 ck (genv,env) s1 e1 (s2, Rval v) /\
-evaluate_i2 ck (genv,opt_bind n v env) s2 e2 bv)
+/\ (! ck exh genv env n e1 e2 v bv s1 s2.
+(evaluate_i2 ck (exh,genv,env) s1 e1 (s2, Rval v) /\
+evaluate_i2 ck (exh,genv,opt_bind n v env) s2 e2 bv)
 ==>
-evaluate_i2 ck (genv,env) s1 (Let_i2 n e1 e2) bv)
+evaluate_i2 ck (exh,genv,env) s1 (Let_i2 n e1 e2) bv)
 
 /\ (! ck env n e1 e2 err s s'.
 (evaluate_i2 ck env s e1 (s', Rerr err))
 ==>
 evaluate_i2 ck env s (Let_i2 n e1 e2) (s', Rerr err))
 
-/\ (! ck genv env funs e bv s.
+/\ (! ck exh genv env funs e bv s.
 (ALL_DISTINCT (MAP (\ (x,y,z) .  x) funs) /\
-evaluate_i2 ck (genv,build_rec_env_i2 funs env env) s e bv)
+evaluate_i2 ck (exh,genv,build_rec_env_i2 funs env env) s e bv)
 ==>
-evaluate_i2 ck (genv,env) s (Letrec_i2 funs e) bv)
+evaluate_i2 ck (exh,genv,env) s (Letrec_i2 funs e) bv)
 
 /\ (! ck env funs e s.
 (~ (ALL_DISTINCT (MAP (\ (x,y,z) .  x) funs)))
@@ -774,77 +742,77 @@ evaluate_list_i2 ck env s2 es (s3, Rerr err))
 ==>
 evaluate_list_i2 ck env s1 (e::es) (s3, Rerr err))
 
-/\ (! ck env v s.
+/\ (! ck env v s err_v.
 T
 ==>
-evaluate_match_i2 ck env s v [] (s, Rerr Rtype_error))
+evaluate_match_i2 ck env s v [] err_v (s, Rerr (Rraise err_v)))
 
-/\ (! ck genv env env' v p pes e bv s count.
+/\ (! ck exh genv env env' v p pes e bv s count err_v.
 (ALL_DISTINCT (pat_bindings_i2 p []) /\
-((pmatch_i2 s p v env = Match env') /\
-evaluate_i2 ck (genv,env') (count,s) e bv))
+((pmatch_i2 exh s p v env = Match env') /\
+evaluate_i2 ck (exh,genv,env') (count,s) e bv))
 ==>
-evaluate_match_i2 ck (genv,env) (count,s) v ((p,e)::pes) bv)
+evaluate_match_i2 ck (exh,genv,env) (count,s) v ((p,e)::pes) err_v bv)
 
-/\ (! ck genv env v p e pes bv s count.
+/\ (! ck exh genv env v p e pes bv s count err_v.
 (ALL_DISTINCT (pat_bindings_i2 p []) /\
-((pmatch_i2 s p v env = No_match) /\
-evaluate_match_i2 ck (genv,env) (count,s) v pes bv))
+((pmatch_i2 exh s p v env = No_match) /\
+evaluate_match_i2 ck (exh,genv,env) (count,s) v pes err_v bv))
 ==>
-evaluate_match_i2 ck (genv,env) (count,s) v ((p,e)::pes) bv)
+evaluate_match_i2 ck (exh,genv,env) (count,s) v ((p,e)::pes) err_v bv)
 
-/\ (! ck genv env v p e pes s count.
-(pmatch_i2 s p v env = Match_type_error)
+/\ (! ck exh genv env v p e pes s count err_v.
+(pmatch_i2 exh s p v env = Match_type_error)
 ==>
-evaluate_match_i2 ck (genv,env) (count,s) v ((p,e)::pes) ((count,s), Rerr Rtype_error))
+evaluate_match_i2 ck (exh,genv,env) (count,s) v ((p,e)::pes) err_v ((count,s), Rerr Rtype_error))
 
-/\ (! ck env v p e pes s.
+/\ (! ck env v p e pes s err_v.
 (~ (ALL_DISTINCT (pat_bindings_i2 p [])))
 ==>
-evaluate_match_i2 ck env s v ((p,e)::pes) (s, Rerr Rtype_error))`;
+evaluate_match_i2 ck env s v ((p,e)::pes) err_v (s, Rerr Rtype_error))`;
 
-val _ = Hol_reln ` (! ck genv n e vs s1 s2.
-(evaluate_i2 ck (genv,emp) s1 e (s2, Rval (Conv_i2 tuple_tag vs)) /\
+val _ = Hol_reln ` (! ck exh genv n e vs s1 s2.
+(evaluate_i2 ck (exh,genv,emp) s1 e (s2, Rval (Conv_i2 (tuple_tag,NONE) vs)) /\
 (LENGTH vs = n))
 ==>
-evaluate_dec_i2 ck genv s1 (Dlet_i2 n e) (s2, Rval vs))
+evaluate_dec_i2 ck exh genv s1 (Dlet_i2 n e) (s2, Rval vs))
 
-/\ (! ck genv n e vs s1 s2.
-(evaluate_i2 ck (genv,emp) s1 e (s2, Rval (Conv_i2 tuple_tag vs)) /\ ~ ((LENGTH vs) = n))
+/\ (! ck exh genv n e vs s1 s2.
+(evaluate_i2 ck (exh,genv,emp) s1 e (s2, Rval (Conv_i2 (tuple_tag,NONE) vs)) /\ ~ ((LENGTH vs) = n))
 ==>
-evaluate_dec_i2 ck genv s1 (Dlet_i2 n e) (s2, Rerr Rtype_error))
+evaluate_dec_i2 ck exh genv s1 (Dlet_i2 n e) (s2, Rerr Rtype_error))
 
-/\ (! ck genv n e v s1 s2.
-(evaluate_i2 ck (genv,emp) s1 e (s2, Rval v) /\
-~ (? vs. v = Conv_i2 tuple_tag vs))
+/\ (! ck exh genv n e v s1 s2.
+(evaluate_i2 ck (exh,genv,emp) s1 e (s2, Rval v) /\
+~ (? vs. v = Conv_i2 (tuple_tag,NONE) vs))
 ==>
-evaluate_dec_i2 ck genv s1 (Dlet_i2 n e) (s2, Rerr Rtype_error))
+evaluate_dec_i2 ck exh genv s1 (Dlet_i2 n e) (s2, Rerr Rtype_error))
 
-/\ (! ck genv n e err s s'.
-(evaluate_i2 ck (genv,emp) s e (s', Rerr err))
+/\ (! ck exh genv n e err s s'.
+(evaluate_i2 ck (exh,genv,emp) s e (s', Rerr err))
 ==>
-evaluate_dec_i2 ck genv s (Dlet_i2 n e) (s', Rerr err))
+evaluate_dec_i2 ck exh genv s (Dlet_i2 n e) (s', Rerr err))
 
-/\ (! ck genv funs s.
+/\ (! ck exh genv funs s.
 T
 ==>
-evaluate_dec_i2 ck genv s (Dletrec_i2 funs) (s, Rval (MAP (\ (f,x,e) .  Closure_i2 [] x e) funs)))`;
+evaluate_dec_i2 ck exh genv s (Dletrec_i2 funs) (s, Rval (MAP (\ (f,x,e) .  Closure_i2 [] x e) funs)))`;
 
-val _ = Hol_reln ` (! ck genv s.
+val _ = Hol_reln ` (! ck exh genv s.
 T
 ==>
-evaluate_decs_i2 ck genv s [] (s, [], NONE))
+evaluate_decs_i2 ck exh genv s [] (s, [], NONE))
 
-/\ (! ck s1 s2 genv d ds e.
-(evaluate_dec_i2 ck genv s1 d (s2, Rerr e))
+/\ (! ck exh s1 s2 genv d ds e.
+(evaluate_dec_i2 ck exh genv s1 d (s2, Rerr e))
 ==>
-evaluate_decs_i2 ck genv s1 (d::ds) (s2, [], SOME e))
+evaluate_decs_i2 ck exh genv s1 (d::ds) (s2, [], SOME e))
 
-/\ (! ck s1 s2 s3 genv d ds new_env new_env' r.
-(evaluate_dec_i2 ck genv s1 d (s2, Rval new_env) /\
-evaluate_decs_i2 ck (genv ++ MAP SOME new_env) s2 ds (s3, new_env', r))
+/\ (! ck exh s1 s2 s3 genv d ds new_env new_env' r.
+(evaluate_dec_i2 ck exh genv s1 d (s2, Rval new_env) /\
+evaluate_decs_i2 ck exh (genv ++ MAP SOME new_env) s2 ds (s3, new_env', r))
 ==>
-evaluate_decs_i2 ck genv s1 (d::ds) (s3, (new_env ++ new_env'), r))`;
+evaluate_decs_i2 ck exh genv s1 (d::ds) (s3, (new_env ++ new_env'), r))`;
 
  val _ = Define `
 
@@ -855,45 +823,45 @@ evaluate_decs_i2 ck genv s1 (d::ds) (s3, (new_env ++ new_env'), r))`;
 (num_defs (Dletrec_i2 funs::ds) = (LENGTH funs + num_defs ds))`;
 
 
-val _ = Hol_reln ` (! ck genv s1 ds s2 env.
-(evaluate_decs_i2 ck genv s1 ds (s2,env,NONE))
+val _ = Hol_reln ` (! ck exh genv s1 ds s2 env.
+(evaluate_decs_i2 ck exh genv s1 ds (s2,env,NONE))
 ==>
-evaluate_prompt_i2 ck genv s1 (Prompt_i2 ds) (s2, MAP SOME env, NONE))
+evaluate_prompt_i2 ck exh genv s1 (Prompt_i2 ds) (s2, MAP SOME env, NONE))
 
-/\ (! ck genv s1 ds s2 env err.
-(evaluate_decs_i2 ck genv s1 ds (s2,env,SOME err))
+/\ (! ck exh genv s1 ds s2 env err.
+(evaluate_decs_i2 ck exh genv s1 ds (s2,env,SOME err))
 ==>
-evaluate_prompt_i2 ck genv s1 (Prompt_i2 ds) (s2,                                           
+evaluate_prompt_i2 ck exh genv s1 (Prompt_i2 ds) (s2,                                           
  (MAP SOME env ++ GENLIST (\n .  
   (case (n ) of ( _ ) => NONE )) (num_defs ds - LENGTH env)),
                                            SOME err))`;
 
-val _ = Hol_reln ` (! ck genv s.
+val _ = Hol_reln ` (! ck exh genv s.
 T
 ==>
-evaluate_prog_i2 ck genv s [] (s, [], NONE))
+evaluate_prog_i2 ck exh genv s [] (s, [], NONE))
 
-/\ (! ck genv s1 prompt prompts s2 env2 s3 env3 r.
-(evaluate_prompt_i2 ck genv s1 prompt (s2, env2, NONE) /\
-evaluate_prog_i2 ck (genv++env2) s2 prompts (s3, env3, r))
+/\ (! ck exh genv s1 prompt prompts s2 env2 s3 env3 r.
+(evaluate_prompt_i2 ck exh genv s1 prompt (s2, env2, NONE) /\
+evaluate_prog_i2 ck exh (genv++env2) s2 prompts (s3, env3, r))
 ==>
-evaluate_prog_i2 ck genv s1 (prompt::prompts) (s3, (env2++env3), r))
+evaluate_prog_i2 ck exh genv s1 (prompt::prompts) (s3, (env2++env3), r))
 
-/\ (! ck genv s1 prompt prompts s2 env2 err.
-(evaluate_prompt_i2 ck genv s1 prompt (s2, env2, SOME err))
+/\ (! ck exh genv s1 prompt prompts s2 env2 err.
+(evaluate_prompt_i2 ck exh genv s1 prompt (s2, env2, SOME err))
 ==>
-evaluate_prog_i2 ck genv s1 (prompt::prompts) (s2, env2, SOME err))`;
+evaluate_prog_i2 ck exh genv s1 (prompt::prompts) (s2, env2, SOME err))`;
 
 (*val init_tagenv_state : (nat * tag_env * map nat (conN * tid_or_exn))*)
 val _ = Define `
  (init_tagenv_state =
   ( 6,
    (FEMPTY,
-    FUPDATE_LIST FEMPTY [("Div", (div_tag, NONE)); 
-                  ("Bind", (bind_tag,NONE)); 
-                  ("Eq", (eq_tag, NONE)); 
-                  ("::", (cons_tag, SOME ["::"; "nil"]));
-                  ("nil", (nil_tag, SOME ["::"; "nil"]))]),
+    FUPDATE_LIST FEMPTY [("Div", (div_tag, SOME (TypeExn (Short "Div")))); 
+                  ("Bind", (bind_tag,SOME (TypeExn (Short "Bind")))); 
+                  ("Eq", (eq_tag, SOME (TypeExn (Short "Eq")))); 
+                  ("::", (cons_tag, SOME (TypeId (Short "list"))));
+                  ("nil", (nil_tag, SOME (TypeId (Short "list"))))]),
    FUPDATE_LIST FEMPTY [(div_tag, ("Div", TypeExn (Short "Div"))); 
                  (bind_tag, ("Bind", TypeExn (Short "Bind"))); 
                  (eq_tag, ("Eq", TypeExn (Short "Eq"))); 
